MiniYul/AlphaEquiv_Correct.thy
@@ -968,107 +968,13 @@ next
     by(auto)
 qed
 
-(* alternative version of varmap_extend that leads to cleaner
- * inductive proof *)
-(*
-fun varmap_extend_alt :: "varmap \<Rightarrow> name list \<Rightarrow> varmap" where
-"varmap_extend_alt vm [] = vm"
-| "varmap_extend_alt vm (nh # nt) =
-   varmap_insert (varmap_extend vm nt) nh 0"
-
-lemma varmap_extend_alt_spec : 
-  assumes "distinct ns"
-  shows "varmap_extend vm ns = varmap_extend_alt vm ns"
-  using assms
-proof(induction ns arbitrary: vm)
-  case Nil
-  then show ?case by auto
-next
-  case (Cons nh nt)
-  show ?case using Cons.prems
-    apply(auto)
-    using sym[OF Cons.IH[of "varmap_insert vm nh 0"]] Cons.IH[of vm]
-    apply(auto)
-
-qed
-*)
-
-(*
-lemma alpha_equiv_varmap'_update_fresh_present :
-  assumes "alpha_equiv_varmap' subst' vm1' vm2'"
-  assumes "oalist_one_one subst'"
-  assumes "oalist_keys subst' = oalist_keys vm1'"
-  assumes "oalist_keys (oalist_flip subst') = oalist_keys vm2'"
-  assumes "n1 \<in> set (oalist_keys vm1')"
-  assumes "n2 \<in> set (oalist_keys vm2')"  
-  shows "alpha_equiv_varmap' (update n1 n2 subst') vm1' vm2'"
-  using assms
-proof(transfer)
-  fix subst'
-  show "\<And> vm1' vm2' n1 n2. strict_order (map fst subst') \<Longrightarrow>
-       strict_order (map fst vm1') \<Longrightarrow>
-       strict_order (map fst vm2') \<Longrightarrow>
-       alpha_equiv_varmap'l subst' vm1' vm2' \<Longrightarrow>
-       distinct (map snd subst') \<Longrightarrow>
-       map fst subst' = map fst vm1' \<Longrightarrow>
-       map fst (oalist_flip' subst') = map fst vm2' \<Longrightarrow> n1 \<in> set (map fst vm1') \<Longrightarrow> n2 \<in> set (map fst vm2') \<Longrightarrow> alpha_equiv_varmap'l (str_ord_update n1 n2 subst') vm1' vm2'"
-  proof(induction subst')
-    case Nil
-    then show ?case
-      by(auto)
-  next
-    case (Cons subst'h subst't)
-
-    obtain hn1 hn2 where Subst'h :
-      "subst'h = (hn1, hn2)"
-      by(cases subst'h; auto)
-
-    obtain val where Val :
-      "map_of vm1' hn1 = Some val" "map_of vm2' hn2 = Some val"
-      "alpha_equiv_varmap'l subst't vm1' vm2'"
-      using Cons.prems Subst'h
-      by(auto split: option.splits)
-
-    obtain val1 where Val1 : "(n1, val1) \<in> set vm1'"
-      using Cons.prems
-      by(auto)
-
-    then have Val1' : "map_of vm1' n1 = Some val1"
-      using Some_eq_map_of_iff[of vm1'] strict_order_distinct[OF Cons.prems(2)]
-      by auto
-
-    obtain val2 where Val2 : "(n2, val2) \<in> set vm2'"
-      using Cons.prems
-      by(auto)
-
-    then have Val2' : "map_of vm2' n2 = Some val2"
-      using Some_eq_map_of_iff[of vm2'] strict_order_distinct[OF Cons.prems(3)]
-      by(auto)
-
-    show ?case
-    proof(cases "n1 = hn1")
-      case True1 : True
-
-
-      show ?thesis using Cons.prems Subst'h
-          True1 Val Val2'
-        apply(auto)
-    next
-      case False1 : False
-      show ?thesis
-      proof(cases "n2 = hn2")
-        case True2 : True
-
-      using Cons.prems Subst'h Val Val1' Val2'
-      apply(auto)
-
-  qed
-*)
+(* strengthen the theorem to talk about subsets of keys? *)
 lemma alpha_equiv_varmap'_update_fresh :
   assumes "alpha_equiv_varmap' subst' vm1' vm2'"
   assumes "oalist_one_one subst'"
-  assumes "oalist_keys subst' = oalist_keys vm1'"
-  assumes "oalist_keys (oalist_flip subst') = oalist_keys vm2'"
+  assumes "set (oalist_keys subst') \<subseteq> set (oalist_keys vm1')"
+  assumes "set (oalist_keys (oalist_flip subst')) \<subseteq> set (oalist_keys vm2')"
+  assumes "n1 \<notin> set (oalist_keys vm1')"
   assumes "n2 \<notin> set (oalist_keys vm2')"
   shows "alpha_equiv_varmap' (update n1 n2 subst') (update n1 v vm1') (update n2 v vm2')"
   using assms
@@ -1080,8 +986,9 @@ proof(transfer)
        strict_order (map fst vm2') \<Longrightarrow>
        alpha_equiv_varmap'l subst' vm1' vm2' \<Longrightarrow>
        distinct (map snd subst') \<Longrightarrow>
-       map fst subst' = map fst vm1' \<Longrightarrow>
-       map fst (oalist_flip' subst') = map fst vm2' \<Longrightarrow>
+       set (map fst subst') \<subseteq> set (map fst vm1') \<Longrightarrow>
+       set (map fst (oalist_flip' subst')) \<subseteq> set (map fst vm2') \<Longrightarrow>
+       n1 \<notin> set (map fst vm1') \<Longrightarrow>
        n2 \<notin> set (map fst vm2') \<Longrightarrow>
        alpha_equiv_varmap'l (str_ord_update n1 n2 subst')
         (str_ord_update n1 v vm1') (str_ord_update n2 v vm2')"
@@ -1135,10 +1042,21 @@ proof(transfer)
         using strict_order_distinct[OF Cons.prems(1)] Subst'h True1
         by(auto)
 
-      show ?thesis using Cons.prems Subst'h
-          Get1_hn1 Get2_n2 True1 Val Ord_tl Val
-        using alpha_equiv_varmap'_update_miss[of vm1' vm2' subst't n1] Notin1
-        apply(auto)
+      show ?thesis
+      proof(cases "n2 = hn2")
+        case True2 : True
+
+        show ?thesis using Cons.prems Subst'h
+            Get1_hn1 Get2_n2 True1 Val Ord_tl Val True1 True2
+          using alpha_equiv_varmap'_update_miss[of vm1' vm2' subst't n1] Notin1
+          by(auto)
+      next
+        case False2 : False
+
+        show ?thesis using Cons.prems Subst'h
+            Get1_hn1 Get2_n2 True1 Val Ord_tl Val True1 False2
+          by(auto)
+      qed
     next
       case False1 : False
       show ?thesis
@@ -1150,12 +1068,12 @@ proof(transfer)
             Get1_hn1 Get2_n2 False1 True2 Val Ord_tl Val
           by(auto)
 
-        have Vm2 : "map fst (str_ord_update hn2 hn1 (oalist_flip' subst't)) = map fst vm2'"
+        have Vm2 : "set (map fst (str_ord_update hn2 hn1 (oalist_flip' subst't))) \<subseteq> set (map fst vm2')"
           using Cons.prems Subst'h
             Get1_hn1 Get2_n2 Val Ord_tl Val
           by(auto)
 
-        have Vm2' : "fst ` set (str_ord_update hn2 hn1 (oalist_flip' subst't)) = fst ` set vm2'"
+        have Vm2' : "fst ` set (str_ord_update hn2 hn1 (oalist_flip' subst't)) \<subseteq> fst ` set vm2'"
           unfolding sym[OF set_map]
           using Vm2
           by(auto)
@@ -1166,7 +1084,7 @@ proof(transfer)
           by auto
 
         have Bad : "(hn2) \<in>  fst ` set vm2'"
-          using Vm2'_set unfolding sym[OF Vm2']
+          using Vm2'_set Vm2'
           by(auto)
 
         show ?thesis using Bad Notin2
@@ -1186,14 +1104,13 @@ proof(transfer)
             using Cons.prems Subst'h False1 strict_order_distinct[OF Cons.prems(1)]
             by(auto)
 
-          have Keys1_alt : "fst ` set (subst'h # subst't) = fst ` set vm1'"
+          have Keys1_alt : "fst ` set (subst'h # subst't) \<subseteq> fst ` set vm1'"
             using Cons.prems
             unfolding sym[OF set_map]
             by auto
 
           have Notin1_alt : "n1 \<notin> fst ` set (subst'h # subst't)"
-            using Notin1
-            unfolding Keys1_alt
+            using Notin1 Keys1_alt
             by(auto)
 
           have Notin1_alt_tl : "n1 \<notin> fst ` set (subst't)"
@@ -1204,14 +1121,13 @@ proof(transfer)
             using Cons.prems Subst'h False1
             by(auto)
 
-          have Keys2_alt : "fst ` set ((oalist_flip' (subst'h # subst't))) = fst ` (set vm2')"
+          have Keys2_alt : "fst ` set ((oalist_flip' (subst'h # subst't))) \<subseteq> fst ` (set vm2')"
             using Cons.prems
             unfolding sym[OF set_map]
             by auto
 
           have Notin2_alt : "n2 \<notin> fst ` set ((oalist_flip' (subst'h # subst't))) "
-            using Notin2
-            unfolding Keys2_alt
+            using Notin2 Keys2_alt
             by(auto)
 
           hence Notin2_alt2 : "n2 \<notin> fst ` (\<lambda>(x, y). (y, x)) ` set (subst'h # subst't)"
@@ -1234,9 +1150,14 @@ proof(transfer)
             using Notin2_alt3
             by auto
 
+          have Get1_hn1' : "map_of (str_ord_update n1 v vm1') hn1 = Some val"
+            using str_ord_update_get_neq[OF Cons.prems(2), of n1 hn1 v] False1
+            using Val
+            by auto
+
           show ?thesis using Cons.prems Subst'h False1 False2 True3
-              Get1_hn1 Get2_n2 False1 False2 Val Get2_miss
-            using alpha_equiv_varmap'_update_miss[OF Cons.prems(2) Cons.prems(3) Ord_tl _ Notin1_alt_tl Notin2_alt_tl]
+              Get1_n1 Get1_hn1' Get1_hn1 Get2_n2 False1 False2 Val Get2_miss
+            using alpha_equiv_varmap'_update_miss[OF Cons.prems(2) Cons.prems(3) Ord_tl _ Notin1_alt_tl Notin2_alt_tl, of v]
             by(auto)
         next
           case False3 : False
@@ -1253,172 +1174,299 @@ proof(transfer)
             using Cons.prems Subst'h False1 strict_order_distinct[OF Cons.prems(1)]
             by(auto)
 
-          obtain vm1'hk vm1'hv vm1't where Vm1'_cons : "vm1' = (vm1'hk, vm1'hv) # vm1't"
-            using Cons.prems
-            by(cases vm1'; auto)
+          have Get1_hn1' : "map_of (str_ord_update n1 v vm1') hn1 = Some val"
+            using str_ord_update_get_neq[OF Cons.prems(2), of n1 hn1 v] False1
+            using Val
+            by auto
 
-          have Vm_tl' : "alpha_equiv_varmap'l subst't ((vm1'hk, val) # vm1't) vm2'"
-            using Cons.prems Subst'h False1 False2 False3
-              Get1_hn1 Get2_n2 Get2_miss Val Lt Vm1'_cons
-            by(auto)
+          have Fst_flip : "fst o (\<lambda>(x, y). (y, x)) = snd"
+          proof
+            fix w
+            show "(fst \<circ> (\<lambda>(x, y). (y, x))) w = snd w"
+              by(cases w; auto)
+          qed
+
+          have Vm2'_superset : "fst ` set (oalist_flip' (subst'h # subst't)) \<subseteq> fst ` set vm2'"
+            using Cons.prems
+            by auto
+
+          have Flip_set : "set (oalist_flip' (subst'h # subst't)) = 
+            (\<lambda>(x, y). (y, x)) ` set (subst'h # subst't)"
+            using oalist_flip'_set[OF Cons.prems(1)] Cons.prems
+            by auto
+
+          have Flip_set' : "set (oalist_flip' (subst't)) = 
+            (\<lambda>(x, y). (y, x)) ` set (subst't)"
+            using oalist_flip'_set[OF Ord_tl] Cons.prems
+            by auto
+
+(*          have Vm2'_superset' :*)
+          have "fst ` (\<lambda>(x, y). (y, x)) ` set (subst'h # subst't) \<subseteq> fst ` set vm2'"
+            using Vm2'_superset unfolding Flip_set
+            by auto
+
+          hence 
+            "snd ` set (subst'h # subst't) \<subseteq> fst ` set vm2'"
+            unfolding image_comp Fst_flip
+            by auto
+
+          hence "snd ` set (subst't) \<subseteq> fst ` set vm2'"
+            by auto
+
+          hence "(fst \<circ> (\<lambda>(x, y). (y, x))) ` set (subst't) \<subseteq> fst ` set vm2'"
+            unfolding sym[OF Fst_flip]
+            by auto
+
+          hence "fst ` (\<lambda>(x, y). (y, x)) ` set (subst't) \<subseteq> fst ` set vm2'"
+            by auto
+
+          hence Vm2_superset' : "fst ` set (oalist_flip' subst't) \<subseteq> fst ` set vm2'"
+            unfolding Flip_set'
+            by auto
 
           show ?thesis using Cons.prems Subst'h False1 False2 False3
-              Get1_hn1 Get2_n2 Get2_miss Val Lt Vm1'_cons
-            apply(auto)
+              Get1_hn1 Get1_hn1' Get2_n2 Get2_miss Val Lt 
+            using Cons.IH[of vm1' vm2' n1 n2 v] Ord_tl Vm2_superset'
+            by(auto)
         qed
-
-        show ?thesis using Cons.prems Subst'h
-            Get1_hn1 Get2_n2 False1 False2 Val Get2_miss
-          apply(auto)
-          sorry
       qed
     qed
   qed
 qed
 
-
-lemma alpha_equiv_varmap'_update_fresh :
-  assumes "alpha_equiv_varmap' subst' vm1' vm2'"
-  assumes "oalist_one_one subst'"
-  assumes "oalist_keys subst' = oalist_keys vm1'"
-  assumes "oalist_keys (oalist_flip subst') = oalist_keys vm2'"
-  assumes "n1 \<notin> set (oalist_keys vm1')"
-  assumes "n2 \<notin> set (oalist_keys vm2')"
-  shows "alpha_equiv_varmap' (update n1 n2 subst') (update n1 v vm1') (update n2 v vm2')"
+lemma oalist_keys_update_eq :
+  fixes l1 :: "('k :: linorder, 'v1) oalist"
+  fixes l2 :: "('k :: linorder, 'v2) oalist"
+  assumes "oalist_keys l1 = oalist_keys l2"
+  shows "oalist_keys (update n v1 l1) = oalist_keys (update n v2 l2)"
   using assms
 proof(transfer)
-  fix subst' 
-  show "\<And>n1 n2 v vm1' vm2'.
-       strict_order (map fst subst') \<Longrightarrow>
-       strict_order (map fst vm1') \<Longrightarrow>
-       strict_order (map fst vm2') \<Longrightarrow>
-       alpha_equiv_varmap'l subst' vm1' vm2' \<Longrightarrow>
-       distinct (map snd subst') \<Longrightarrow>
-       map fst subst' = map fst vm1' \<Longrightarrow>
-       map fst (oalist_flip' subst') = map fst vm2' \<Longrightarrow>
-       n1 \<notin> set (map fst vm1') \<Longrightarrow>
-       n2 \<notin> set (map fst vm2') \<Longrightarrow>
-       alpha_equiv_varmap'l (str_ord_update n1 n2 subst')
-        (str_ord_update n1 v vm1') (str_ord_update n2 v vm2')"
-  proof(induction subst')
+  fix l1 :: "('k :: linorder * 'v1) list"
+  show "\<And> (l2 :: ('k :: linorder * 'v2) list) n v1 v2 .
+       strict_order (map fst l1) \<Longrightarrow>
+       strict_order (map fst l2) \<Longrightarrow>
+       map fst l1 = map fst l2 \<Longrightarrow>
+       map fst (str_ord_update n v1 l1) = map fst (str_ord_update n v2 l2)"
+  proof(induction l1)
     case Nil
     then show ?case 
       by(auto)
   next
-    case (Cons subst'h subst't)
+    case (Cons l1h l1t)
 
-    obtain hn1 hn2 where Subst'h :
-      "subst'h = (hn1, hn2)"
-      by(cases subst'h; auto)
+    obtain hk l1hv where L1h : "l1h = (hk, l1hv)"
+      by(cases l1h; auto)
 
-    have Get1_hn1 : "map_of (str_ord_update hn1 v vm1') hn1 = Some v"
-      using str_ord_update_get_eq[OF Cons.prems(2)]
-      by(auto)
+    obtain l2h l2t where Cons' : "l2 = l2h # l2t"
+      using Cons.prems
+      by(cases l2; auto)
 
-    have Get2_n2 : "map_of (str_ord_update n2 v vm2') n2 = Some v"
-      using str_ord_update_get_eq[OF Cons.prems(3)]
-      by(auto)
-
-    have Get1_n1 : "map_of (str_ord_update n1 v vm1') n1 = Some v"
-      using str_ord_update_get_eq[OF Cons.prems(2)]
-      by(auto)
-
-    have Ord_tl : "strict_order (map fst subst't)"
-      using Cons.prems strict_order_tl
-      by auto
-
-    obtain val where Val :
-      "map_of vm1' hn1 = Some val" "map_of vm2' hn2 = Some val"
-      "alpha_equiv_varmap'l subst't vm1' vm2'"
-      using Cons.prems Subst'h
-      by(auto split: option.splits)
-
+    obtain l2hv where L2h : "l2h = (hk, l2hv)"
+      using Cons.prems L1h Cons'
+      by(cases l2h; auto)
 
     show ?case
-    proof(cases "n1 = hn1")
-      case True1 : True
+    proof(cases "hk < n")
+      case True
 
-      show ?thesis using Cons.prems Subst'h
-          Get1_hn1 Get2_n2 True1 Val Ord_tl Val
+      have Ord_tl1 : "strict_order (map fst l1t)"
+        using strict_order_tl Cons.prems
+        by auto
+
+      have Ord_tl2 : "strict_order (map fst l2t)"
+        using strict_order_tl Cons.prems Cons'
+        by auto
+
+      show ?thesis 
+        using Cons.prems L1h Cons' L2h True
+        using Cons.IH[OF Ord_tl1 Ord_tl2]
         by(auto)
     next
-      case False1 : False
+      case False
+      then show ?thesis using Cons.prems L1h Cons' L2h
+        by(auto)
+    qed
+  qed
+qed
+
+lemma oalist_flip_update : 
+  fixes l :: "('k :: linorder, 'k) oalist"
+  assumes "oalist_one_one l"
+  assumes "k \<notin> set (oalist_keys l)"
+  assumes "v \<notin> set (oalist_keys (oalist_flip l))"
+  shows "oalist_flip (update k v l) = update v k (oalist_flip l)"
+  using assms
+proof(transfer)
+  fix l :: "('k :: linorder * 'k) list"
+  fix k v
+  assume Ord : "strict_order (map fst l)"
+  assume Dist : "distinct (map snd l)"
+  assume Notin1 : "k \<notin> set (map fst l)"
+  assume Notin2 : "v \<notin> set (map fst (oalist_flip' l))"
+
+  have Notin1' : "k \<notin> fst ` set l"
+    using Notin1 by auto
+
+  have Fst_flip : "fst o (\<lambda>(x, y). (y, x)) = snd"
+  proof
+    fix w
+    show "(fst \<circ> (\<lambda>(x, y). (y, x))) w = snd w"
+      by(cases w; auto)
+  qed
+
+
+  have Notin2_alt : "v \<notin> fst ` set (oalist_flip' l)"
+    using Notin2
+    by auto
+
+  hence "v \<notin> fst ` (\<lambda>(x, y). (y, x)) ` set l"
+    using oalist_flip'_set[OF Ord Dist]
+    by auto
+
+  hence "v \<notin> (fst o (\<lambda>(x, y). (y, x))) ` set l"
+    by auto
+
+  hence Notin2' : "v \<notin> snd ` set l"
+    unfolding Fst_flip by auto
+
+  show "oalist_flip' (str_ord_update k v l) = str_ord_update v k (oalist_flip' l)"
+    using oalist_flip'_update[OF Ord Dist Notin1' Notin2']
+    by auto
+qed
+
+lemma oalist_one_one_update : 
+  fixes l :: "('k :: linorder, 'k) oalist"
+  assumes "oalist_one_one l"
+  assumes "k \<notin> set (oalist_keys l)"
+  assumes "v \<notin> set (oalist_keys (oalist_flip l))"
+  shows "oalist_one_one (update k v l)"
+  using assms
+proof(transfer)
+  fix l :: "('k * 'k) list"
+  show "\<And> v k.
+       strict_order (map fst l) \<Longrightarrow>
+       distinct (map snd l) \<Longrightarrow>
+       k \<notin> set (map fst l) \<Longrightarrow>
+       v \<notin> set (map fst (oalist_flip' l)) \<Longrightarrow> distinct (map snd (str_ord_update k v l))"
+  proof(induction l)
+    case Nil
+    then show ?case
+      by(auto)
+  next
+    case (Cons lh lt)
+
+    obtain lhk lhv where Lh : "lh = (lhk, lhv)"
+      by(cases lh; auto)
+
+    have Ord_tl : "strict_order (map fst lt)"
+      using strict_order_tl Cons.prems
+      by auto
+
+    show ?case
+    proof(cases "k < lhk")
+      case K_lt : True
+
       show ?thesis
-      proof(cases "n2 = hn2")
-        case True2 : True
+      proof(cases "v = lhv")
+        case V_eq : True
 
-        have Notin2: "hn2 \<notin> fst ` set vm2'"
-          using Cons.prems Subst'h
-            Get1_hn1 Get2_n2 False1 True2 Val Ord_tl Val
+        have Lhv_notin : "lhv \<notin> fst ` set (str_ord_update lhv lhk (oalist_flip' lt))"
+          using Cons Lh K_lt V_eq
           by(auto)
 
-        have Vm2 : "map fst (str_ord_update hn2 hn1 (oalist_flip' subst't)) = map fst vm2'"
-          using Cons.prems Subst'h
-            Get1_hn1 Get2_n2 Val Ord_tl Val
-          by(auto)
-
-        have Vm2' : "fst ` set (str_ord_update hn2 hn1 (oalist_flip' subst't)) = fst ` set vm2'"
-          unfolding sym[OF set_map]
-          using Vm2
-          by(auto)
-
-        have Vm2'_set : "set (str_ord_update hn2 hn1 (oalist_flip' subst't)) =
-          set (oalist_flip' subst't) - { x . fst x = hn2 } \<union> {(hn2, hn1)}"
-          using str_ord_update_set[OF oalist_flip'_correct[OF Ord_tl]]
+        then have Lhv_notin' : "lhv \<notin> fst ` (set (oalist_flip' lt) - {x. fst x = lhv} \<union> {(lhv, lhk)})"
+          using str_ord_update_set[OF oalist_flip'_correct[OF Ord_tl], of lhv lhk]
           by auto
 
-        have Bad : "(hn2) \<in>  fst ` set vm2'"
-          using Vm2'_set unfolding sym[OF Vm2']
-          by(auto)
-
-        show ?thesis using Bad Notin2
+        then have False
           by auto
+
+        then show ?thesis by auto
       next
-        case False2 : False
+        case V_neq : False
 
-        have Get2_miss : "map_of (str_ord_update n2 v vm2') hn2 = Some val"
-          using str_ord_update_get_neq[OF Cons.prems(3) False2, of v] Val
+        have Fst_flip : "fst o (\<lambda>(x, y). (y, x)) = snd"
+        proof
+          fix w
+          show "(fst \<circ> (\<lambda>(x, y). (y, x))) w = snd w"
+            by(cases w; auto)
+        qed
+
+        have V_notin : "v \<notin> fst ` set (str_ord_update lhv lhk (oalist_flip' lt))"
+          using Cons.prems Lh K_lt V_neq
+          by auto
+
+        then have V_notin' : "v \<notin> fst ` (set (oalist_flip' lt) - {x. fst x = lhv} \<union> {(lhv, lhk)})"
+          using str_ord_update_set[OF oalist_flip'_correct[OF Ord_tl], of lhv lhk]
+          by auto
+
+        then have V_notin_tl : "v \<notin> fst ` set (oalist_flip' lt)"
+          by auto
+
+        then have "v \<notin> fst ` (\<lambda>(x, y). (y, x)) ` set lt"
+          using oalist_flip'_set[OF Ord_tl] Cons.prems
+          by auto
+
+        then have "v \<notin> (fst o (\<lambda>(x, y). (y, x))) ` set lt"
+          by auto
+
+        then have "v \<notin> snd ` set lt"
+          unfolding Fst_flip
+          by auto
+
+        then show ?thesis
+          using Cons.prems Lh K_lt V_neq V_notin_tl
           by(auto)
+      qed
+    next
+      case K_nlt : False
+
+      show ?thesis
+      proof(cases "k = lhk")
+        case K_eq : True
+
+        then have False
+          using Cons.prems Lh
+          by auto
+
+        then show ?thesis by auto
+      next
+        case K_gt' : False
+
+        have K_gt : "lhk < k"
+          using K_nlt K_gt'
+          by auto
 
         show ?thesis
-        proof(cases "n1 < hn1")
-          case True3 : True
+        proof(cases "v = lhv")
+          case V_eq : True
+  
+          have Lhv_notin : "lhv \<notin> fst ` set (str_ord_update lhv lhk (oalist_flip' lt))"
+            using Cons Lh V_eq
+            by(auto)
+  
+          then have Lhv_notin' : "lhv \<notin> fst ` (set (oalist_flip' lt) - {x. fst x = lhv} \<union> {(lhv, lhk)})"
+            using str_ord_update_set[OF oalist_flip'_correct[OF Ord_tl], of lhv lhk]
+            by auto
+  
+          then have False
+            by auto
+  
+          then show ?thesis by auto
+        next
+          case V_neq : False
 
-          have Notin1 : "n1 \<notin> fst ` set vm1'"
-            using Cons.prems Subst'h False1 strict_order_distinct[OF Cons.prems(1)]
+          have Lhv_notin : "lhv \<notin> snd ` set lt"
+            using Cons.prems Lh V_neq
             by(auto)
 
-          have Keys1_alt : "fst ` set (subst'h # subst't) = fst ` set vm1'"
-            using Cons.prems
-            unfolding sym[OF set_map]
+          hence "lhv \<notin> snd ` (set lt - {x. fst x = k} \<union> {(k, v)})"
+            using V_neq
             by auto
 
-          have Notin1_alt : "n1 \<notin> fst ` set (subst'h # subst't)"
-            using Notin1
-            unfolding Keys1_alt
-            by(auto)
-
-          have Notin1_alt_tl : "n1 \<notin> fst ` set (subst't)"
-            using Notin1_alt
+          hence Lhv_notin' : "lhv \<notin> snd ` set (str_ord_update k v lt)"
+            using str_ord_update_set[OF Ord_tl]
             by auto
-
-          have Notin2 : "n2 \<notin> fst ` set vm2'"
-            using Cons.prems Subst'h False1
-            by(auto)
-
-          have Keys2_alt : "fst ` set ((oalist_flip' (subst'h # subst't))) = fst ` (set vm2')"
-            using Cons.prems
-            unfolding sym[OF set_map]
-            by auto
-
-          have Notin2_alt : "n2 \<notin> fst ` set ((oalist_flip' (subst'h # subst't))) "
-            using Notin2
-            unfolding Keys2_alt
-            by(auto)
-
-          hence Notin2_alt2 : "n2 \<notin> fst ` (\<lambda>(x, y). (y, x)) ` set (subst'h # subst't)"
-            using oalist_flip'_set[OF Cons.prems(1)] Cons.prems
-            by(auto)
 
           have Fst_flip : "fst o (\<lambda>(x, y). (y, x)) = snd"
           proof
@@ -1426,126 +1474,429 @@ proof(transfer)
             show "(fst \<circ> (\<lambda>(x, y). (y, x))) w = snd w"
               by(cases w; auto)
           qed
-
-          have Notin2_alt3 : "n2 \<notin> snd ` set (subst'h # subst't)"
-            using Notin2_alt2
-            unfolding image_comp Fst_flip
-            by(auto)
-
-          have Notin2_alt_tl : "n2 \<notin> snd ` set (subst't)"
-            using Notin2_alt3
+  
+          have V_notin : "v \<notin> fst ` set (str_ord_update lhv lhk (oalist_flip' lt))"
+            using Cons.prems Lh V_neq
             by auto
-
-          show ?thesis using Cons.prems Subst'h False1 False2 True3
-              Get1_hn1 Get2_n2 False1 False2 Val Get2_miss
-            using alpha_equiv_varmap'_update_miss[OF Cons.prems(2) Cons.prems(3) Ord_tl _ Notin1_alt_tl Notin2_alt_tl]
+  
+          then have V_notin' : "v \<notin> fst ` (set (oalist_flip' lt) - {x. fst x = lhv} \<union> {(lhv, lhk)})"
+            using str_ord_update_set[OF oalist_flip'_correct[OF Ord_tl], of lhv lhk]
+            by auto
+  
+          then have V_notin_tl : "v \<notin> fst ` set (oalist_flip' lt)"
+            by auto
+  
+  
+          show ?thesis
+            using Cons.prems Lh K_gt V_neq Lhv_notin'
+            using Cons.IH[OF Ord_tl, of k v] V_notin_tl
             by(auto)
-        next
-          case False3 : False
-
-          have Lt : "hn1 < n1"
-            using False1 False2 False3
-            by(auto)
-
-          have Notin1 : "n1 \<notin> set (map fst vm1')"
-            using Cons.prems Subst'h False1 strict_order_distinct[OF Cons.prems(1)]
-            by(auto)
-
-          have Notin2 : "n2 \<notin> set (map fst vm2')"
-            using Cons.prems Subst'h False1 strict_order_distinct[OF Cons.prems(1)]
-            by(auto)
-
-          obtain vm1'hk vm1'hv vm1't where Vm1'_cons : "vm1' = (vm1'hk, vm1'hv) # vm1't"
-            using Cons.prems
-            by(cases vm1'; auto)
-
-          have Vm_tl' : "alpha_equiv_varmap'l subst't ((vm1'hk, val) # vm1't) vm2'"
-            using Cons.prems Subst'h False1 False2 False3
-              Get1_hn1 Get2_n2 Get2_miss Val Lt Vm1'_cons
-            by(auto)
-
-          show ?thesis using Cons.prems Subst'h False1 False2 False3
-              Get1_hn1 Get2_n2 Get2_miss Val Lt Vm1'_cons
-              Cons.IH
-            apply(auto)
         qed
-
-        show ?thesis using Cons.prems Subst'h
-            Get1_hn1 Get2_n2 False1 False2 Val Get2_miss
-          apply(auto)
-          sorry
       qed
     qed
   qed
 qed
 
-
-(* need assumptions about n1 and n2 not being present in substh? 
- * no, I think we need them to not be present in vm1h *)
 lemma alpha_equiv_varmap_insert :
-  assumes "alpha_equiv_varmap (substh # substt) vm1 vm2"
-  shows "alpha_equiv_varmap (update n1 n2 substh # substt)
-     (varmap_insert vm1 n1 v)
-     (varmap_insert vm2 n2 v)"
+  assumes Heqv : "alpha_equiv_varmap (substh # substt) (vm1h # vm1t) (vm2h # vm2t)"
+  assumes Hone_one : "oalist_one_one substh"
+  assumes Hkeys1 : "oalist_keys substh = oalist_keys vm1h"
+  assumes Hkeys2 : "oalist_keys (oalist_flip substh) = oalist_keys vm2h"
+  assumes N1_notin : "n1 \<notin> set (oalist_keys vm1h)"
+  assumes N2_notin : "n2 \<notin> set (oalist_keys vm2h)"
+  shows "alpha_equiv_varmap (update n1 n2 substh # substt) (varmap_insert (vm1h # vm1t) n1 v) (varmap_insert (vm2h # vm2t) n2 v)"
   using assms
-proof(induction substt arbitrary: substh vm1 vm2 n1 n2 v)
-  case Nil
-  then show ?case
-    apply(cases vm1; cases vm2; auto)
-    sorry
-next
-  case Cons_s : (Cons sh' st')
+proof-
 
-  obtain vm1h vm1t where Cons1 : "vm1 = vm1h # vm1t"
-    using Cons_s.prems
-    by(cases vm1; auto)
-
-  obtain vm2h vm2t where Cons2 : "vm2 = vm2h # vm2t"
-    using Cons_s.prems
-    by(cases vm2; auto)
-
-  show ?case
-    using Cons_s.prems Cons1 Cons2
-    using Cons_s.IH[of sh' vm1t vm2t]
-    apply(auto)
-
-  have Eq_h : "alpha_equiv_varmap' substh vm1 vm2"
-    using Cons1.prems Cons2
+  have Heqv' : "alpha_equiv_varmap' substh vm1h vm2h"
+    using Heqv
     by auto
 
-  have Conc1 : "alpha_equiv_varmap' (update n1 n2 substh) (update n1 v vm1h) (update n2 v vm2h)"
-    using alpha_equiv_varmap'_update[of "update n1 n2 substh"] (* this won't work *)
-    sorry
+  have Hkeys1' : "set (oalist_keys substh) \<subseteq> set (oalist_keys vm1h)"
+    using Hkeys1 by auto
+
+  have Hkeys2' : "set (oalist_keys (oalist_flip substh)) \<subseteq> set (oalist_keys vm2h)"
+    using Hkeys2 by auto
+
+  have Conc1 : 
+    "alpha_equiv_varmap' (update n1 n2 substh) (update n1 v vm1h) (update n2 v vm2h)"
+    using alpha_equiv_varmap'_update_fresh[OF Heqv' Hone_one Hkeys1' Hkeys2' N1_notin N2_notin]
+    by(auto)
 
   have Conc2 : "oalist_keys (update n1 n2 substh) = oalist_keys (update n1 v vm1h)"
-    sorry
+    using oalist_keys_update_eq[OF Hkeys1]
+    by auto
 
-  have Conc3 : "oalist_one_one (update n1 n2 substh)"
-    sorry
+  have N1_notin_alt : "n1 \<notin> set (oalist_keys substh)"
+    using Hkeys1 N1_notin
+    by auto
 
-  have Conc4 : "oalist_keys (oalist_flip (update n1 n2 substh)) = oalist_keys (update n2 v vm2h)"
-    sorry
+  have N2_notin_alt : "n2 \<notin> set (oalist_keys (oalist_flip substh))"
+    using Hkeys2 N2_notin
+    by auto
 
-  show ?case
-    using Cons1 Cons2 Conc1 Conc2 Conc3 Conc4
+  have Conc3 : "oalist_keys (oalist_flip (update n1 n2 substh)) = oalist_keys (update n2 v vm2h)"
+    using oalist_flip_update[OF Hone_one N1_notin_alt N2_notin_alt]
+    using oalist_keys_update_eq[OF Hkeys2]
+    by(auto)
+
+  have Conc4 : "oalist_one_one (update n1 n2 substh)"
+    using oalist_one_one_update[OF Hone_one, of n1 n2] Hkeys1 Hkeys2 N1_notin N2_notin
+    by auto
+
+  show ?thesis
+    using assms Conc1 Conc2 Conc3 Conc4
     by(auto)
 qed
 
-lemma alpha_equiv_varmap_insert_mini :
-  assumes "length ns1 = length ns2"
-  assumes "alpha_equiv_varmap (to_oalist (zip ns1 ns2) # subst)
-     (varmap_extend (Oalist.empty # vm1) ns1)
-     (varmap_extend (Oalist.empty # vm2) ns2)"
-  shows "alpha_equiv_varmap (update n1 n2 (to_oalist (zip ns1 ns2)) # subst)
-     (varmap_insert (varmap_extend (Oalist.empty # vm1) ns1) n1 0)
-     (varmap_insert (varmap_extend (Oalist.empty # vm2) ns2) n2 0)"
-  using assms
-proof(induction ns1 arbitrary: subst vm1 vm2 n1 n2 ns2)
+lemma oalist_keys_update_set :
+  fixes l :: "('k :: linorder, 'v) oalist"
+  shows "set (oalist_keys (update k v l)) = {k} \<union> set (oalist_keys l)"
+proof(transfer)
+  fix l :: "('k * 'v) list"
+  show "\<And>k v .
+       strict_order (map fst l) \<Longrightarrow>
+       set (map fst (str_ord_update k v l)) = {k} \<union> set (map fst l)"
+  proof(induction l)
+    case Nil
+    then show ?case by auto
+  next
+    case (Cons lh lt)
+
+    obtain lhk lhv where Lh : "lh = (lhk, lhv)"
+      by(cases lh; auto)
+
+    show ?case
+    proof(cases "k < lhk")
+      case K_lt : True
+
+      show ?thesis using Cons Lh K_lt
+        by(auto)
+    next
+      case K_nlt : False
+
+      show ?thesis
+      proof(cases "k = lhk")
+        case K_eq : True
+
+        show ?thesis using Cons Lh K_eq
+          by(auto)
+      next
+        case K_neq : False
+
+        have K_gt : "lhk < k"
+          using K_nlt K_neq
+          by auto
+
+        have Ord_tl : "strict_order (map fst lt)"
+          using strict_order_tl Cons.prems
+          by auto
+
+        show ?thesis
+          using Cons.prems Lh K_gt
+          using Cons.IH[OF Ord_tl]
+          by(auto)
+      qed
+    qed
+  qed
+qed
+
+lemma varmap_extend_keys :
+  shows 
+    "\<exists> vmh' . ((varmap_extend (vmh # vm) ns) = vmh' # vm \<and>
+      set (oalist_keys vmh') = set (oalist_keys vmh) \<union> set ns)"
+proof(induction ns arbitrary: vmh vm)
   case Nil
-  then show ?case
-    apply(auto)
-    sorry
-    
+  then show ?case 
+    by(auto)
+next
+  case (Cons nh nt)
+
+  obtain vmh' where Vmh' : "varmap_extend (update nh 0 vmh # vm) nt = vmh' # vm"
+     "set (oalist_keys vmh') = set (oalist_keys (update nh 0 vmh)) \<union> set nt"
+    using Cons.IH[of "update nh 0 vmh" vm]
+    by(auto)
+
+  have Conc' : "set (oalist_keys (update nh 0 vmh)) \<union> set nt =
+    insert nh (set (oalist_keys vmh) \<union> set nt)"
+    using Vmh'(2) 
+    unfolding oalist_keys_update_set[of nh 0 vmh]
+    by auto
+
+  show ?case using Cons.prems Vmh' Conc'
+    by(simp)
+qed
+
+lemma oalist_keys_empty :
+  "(oalist_keys (Oalist.empty :: (name, int) oalist)) = []"
+  by (transfer; auto)
+
+lemma oalist_keys_empty_nm :
+  "(oalist_keys (Oalist.empty :: (name, name) oalist)) = []"
+  by (transfer; auto)
+
+lemma oalist_one_one_empty :
+  "oalist_one_one (Oalist.empty :: (name, name) oalist)"
+  by(transfer; auto)
+
+lemma str_ord_update_snd_distinct :
+  fixes l :: "('k :: linorder * 'k) list" 
+  assumes "strict_order (map fst l)"
+  assumes "distinct (map snd l)"
+  assumes "k \<notin> set (map fst l)"
+  assumes "v \<notin> set (map snd l)"
+  shows "distinct (map snd (str_ord_update k v l))"
+  using assms
+proof(induction l arbitrary: k v)
+  case Nil
+  then show ?case 
+    by(auto)
+next
+  case (Cons lh lt)
+
+  obtain lhk lhv where Lh :
+    "lh = (lhk, lhv)"
+    by(cases lh; auto)
+
+  have Ord_tl : "strict_order (map fst lt)"
+    using Cons.prems strict_order_tl
+    by auto
+
+  have Notin2' : "lhv \<notin> snd ` set (str_ord_update k v lt)"
+    using Cons.prems Lh
+    using str_ord_update_set[OF Ord_tl]
+    by(auto)
+
+  have Dist_tl : "distinct (map snd (str_ord_update k v lt))"
+    using Cons.prems Lh Cons.IH[OF Ord_tl, of k v]
+    by auto
+
+  show ?case using Cons Lh Notin2' Dist_tl
+    by(auto)
+qed
+
+lemma oalist_one_one_flip : 
+  fixes l :: "('k :: linorder, 'k) oalist" 
+  assumes "oalist_one_one l"
+  shows "oalist_one_one (oalist_flip l)"
+  using assms
+proof(transfer)
+  fix l :: "('k * 'k) list"
+  show "strict_order (map fst l) \<Longrightarrow>
+         distinct (map snd l) \<Longrightarrow> distinct (map snd (oalist_flip' l))"
+    using oalist_flip'_map_snd
+    by auto
+qed
+
+lemma oalist_keys_to_oalist :
+  fixes l :: "(name * name) list"
+  assumes "distinct (map fst l)"
+  shows "set (oalist_keys (to_oalist l)) = set (map fst l)"
+  using assms
+proof(induction l)
+  case Nil
+  then show ?case using oalist_keys_empty_nm
+    by(auto)
+next
+  case (Cons lh lt)
+
+  obtain lhk lhv where Lh :
+    "lh = (lhk, lhv)"
+    by(cases lh; auto)
+
+  show ?case using Cons Lh oalist_keys_update_set[of lhk lhv]
+    by(simp)
+qed
+
+lemma oalist_flip_empty :
+  shows "oalist_flip (empty :: (name, name) oalist) = empty"
+  by(transfer; auto)
+
+lemma oalist_keys_to_oalist_flip_full :
+  fixes l :: "(name * name) list"
+  assumes "distinct (map fst l)"
+  assumes "distinct (map snd l)"
+  shows "set (oalist_keys (oalist_flip (to_oalist l))) = set (map snd l) \<and>
+    oalist_one_one (to_oalist l)"
+  using assms
+proof(induction l)
+  case Nil
+  then show ?case 
+    using oalist_flip_empty oalist_keys_empty_nm oalist_one_one_empty
+    by(auto)
+next
+  case (Cons lh lt)
+
+  obtain lhk lhv where Lh :
+    "lh = (lhk, lhv)"
+    by(cases lh; auto)
+
+  have Ind : "set (oalist_keys (oalist_flip (to_oalist lt))) = set (map snd lt)"
+    "oalist_one_one (to_oalist lt)"
+    using Cons
+    by auto
+
+  have Notin1 : "lhk \<notin> set (oalist_keys (to_oalist lt))"
+    using oalist_keys_to_oalist[of lt] Cons.prems Lh
+    by(auto)
+
+  have Notin2 : "lhv \<notin> set (oalist_keys (oalist_flip (to_oalist lt)))"
+    using Ind Cons.prems Lh
+    by(auto)
+
+  have Flip : "(oalist_flip (update lhk lhv (to_oalist lt))) =
+        update lhv lhk (oalist_flip (to_oalist lt))"
+    using oalist_flip_update[OF Ind(2) Notin1 Notin2]
+    by(auto)
+
+  have Conc1 : "set (oalist_keys (update lhv lhk (oalist_flip (to_oalist lt)))) =
+    insert lhv (snd ` set lt)"
+    unfolding oalist_keys_update_set
+    using Cons
+    by(auto)
+
+  have Conc2 : "oalist_one_one (update lhk lhv (to_oalist lt))"
+    using oalist_one_one_update[OF Ind(2) Notin1 Notin2]
+    by auto
+
+  show ?case using Cons Lh Flip Conc1 Conc2
+    by(clarsimp)
+qed
+
+lemma oalist_keys_to_oalist_flip :
+  fixes l :: "(name * name) list"
+  assumes "distinct (map fst l)"
+  assumes "distinct (map snd l)"
+  shows "set (oalist_keys (oalist_flip (to_oalist l))) = set (map snd l)"
+  using assms oalist_keys_to_oalist_flip_full
+  by auto
+
+lemma to_oalist_one_one :
+  fixes l :: "(name * name) list"
+  assumes "distinct (map fst l)"
+  assumes "distinct (map snd l)"
+  shows "oalist_one_one (to_oalist l)"
+  using assms oalist_keys_to_oalist_flip_full
+  by auto
+
+lemma oalist_flip_flip : 
+  fixes l :: "('k :: linorder, 'k) oalist"
+  assumes "oalist_one_one l"
+  shows "oalist_flip (oalist_flip l) = l"
+  using assms
+proof(transfer)
+  fix l :: "('k * 'k) list"
+  show "strict_order (map fst l) \<Longrightarrow>
+         distinct (map snd l) \<Longrightarrow> oalist_flip' (oalist_flip' l) = l"
+  proof(induction l)
+    case Nil
+    then show ?case by auto
+  next
+    case (Cons lh lt)
+
+    obtain lhk lhv where Lh :
+      "lh = (lhk, lhv)"
+      by(cases lh; auto)
+
+    have Ord_tl : "strict_order (map fst lt)"
+      using strict_order_tl Cons.prems
+      by auto
+
+    have Flip_distinct_tl : " distinct (map snd (oalist_flip' lt))"
+      using oalist_flip'_map_snd[OF Ord_tl] Cons.prems Lh
+      by auto
+
+    have Fst_flip : "fst o (\<lambda>(x, y). (y, x)) = snd"
+    proof
+      fix w
+      show "(fst \<circ> (\<lambda>(x, y). (y, x))) w = snd w"
+        by(cases w; auto)
+    qed
+
+    have Snd_flip : "snd o (\<lambda>(x, y). (y, x)) = fst"
+    proof
+      fix w
+      show "(snd \<circ> (\<lambda>(x, y). (y, x))) w = fst w"
+        by(cases w; auto)
+    qed
+
+    have Flip_set : "set (oalist_flip' lt) = (\<lambda>(x, y). (y, x)) ` set lt"
+      using oalist_flip'_set[OF Ord_tl] Cons.prems Lh
+      by auto
+
+    have Notin1 : "lhv \<notin> snd ` set (lt)"
+      using Cons.prems Lh by auto
+
+    hence "lhv \<notin> (fst o (\<lambda>(x, y). (y, x))) ` set lt"
+      unfolding sym[OF Fst_flip]
+      by auto
+
+    hence "lhv \<notin> fst ` (\<lambda>(x, y). (y, x)) ` set lt"
+      unfolding image_comp
+      by auto
+
+    hence Notin1' : "lhv \<notin> fst ` set (oalist_flip' lt)"
+      using Cons.prems Lh unfolding Flip_set
+      by(auto)
+
+    have Notin2 : "lhk \<notin> fst ` set lt"
+      using strict_order_distinct[OF Cons.prems(1)] Cons.prems Lh
+      by auto
+
+    hence "lhk \<notin> (snd o (\<lambda>(x, y). (y, x))) ` set lt"
+      unfolding sym[OF Snd_flip]
+      by auto
+
+    hence "lhk \<notin> snd ` (\<lambda>(x, y). (y, x)) ` set lt"
+      unfolding image_comp
+      by auto
+
+    hence Notin2' : "lhk \<notin> snd ` set (oalist_flip' lt)"
+      using Cons.prems Lh unfolding Flip_set
+      by(auto)
+
+    have Flip_update : "oalist_flip' (str_ord_update lhv lhk (oalist_flip' lt)) =
+      str_ord_update lhk lhv (oalist_flip' (oalist_flip' lt))"
+      using oalist_flip'_update[OF oalist_flip'_correct[OF Ord_tl] Flip_distinct_tl Notin1' Notin2']
+      using Cons.prems Lh
+      by(auto)
+
+    have Conc' : "str_ord_update lhk lhv lt = (lhk, lhv) # lt"
+    proof(cases lt)
+      case Nil' : Nil
+      then show ?thesis by auto
+    next
+      case Cons' : (Cons lh' lt')
+
+      obtain lh'k lh'v where Lh' : "lh' = (lh'k, lh'v)"
+        by(cases lh'; auto)
+
+      have Lt : "lhk < lh'k"
+        using strict_order_unfold[OF Cons.prems(1), of 1 0]
+        using Lh Cons' Lh'
+        by(auto)
+
+      show ?thesis
+        using Cons' Lh' Lt
+        by(auto)
+    qed
+
+    show ?case using Cons.prems Lh Cons.IH[OF Ord_tl] Flip_update Conc'
+      by(auto)
+  qed
+qed
+
+lemma to_oalist_flip_zip :
+  fixes ns1 ns2 :: "(name) list"
+  assumes "distinct ns1"
+  assumes "distinct ns2"
+  assumes "length ns1 = length ns2"
+  shows "(oalist_flip (to_oalist (zip ns1 ns2))) = to_oalist (zip ns2 ns1)"
+  using assms
+proof(induction ns1 arbitrary: ns2)
+  case Nil
+  then show ?case using oalist_flip_empty oalist_one_one_empty
+    by(auto)
 next
   case Cons1 : (Cons ns1h ns1t)
 
@@ -1553,28 +1904,174 @@ next
     using Cons1.prems
     by(cases ns2; auto)
 
-(*
-  have Eq_h : "alpha_equiv_varmap' substh vm1h vm2h"
-    using Cons1.prems Cons2
+  have Tl : "oalist_flip (to_oalist (zip ns1t ns2t)) = to_oalist (zip ns2t ns1t)"
+    using Cons1.IH[of ns2t] Cons1.prems Cons2
+    by(auto)
+
+  have Dist1' : "distinct (map fst (zip ns1t ns2t))"
+    using map_fst_zip[OF Cons1.prems(3)] Cons1.prems Cons2
     by auto
 
-  have Conc1 : "alpha_equiv_varmap' (update n1 n2 substh) (update n1 v vm1h) (update n2 v vm2h)"
-    using alpha_equiv_varmap'_update[of "update n1 n2 substh"] (* this won't work *)
-    sorry
+  have Dist2' : "distinct (map snd (zip ns1t ns2t))"
+    using map_snd_zip[OF Cons1.prems(3)] Cons1.prems Cons2
+    by auto
 
-  have Conc2 : "oalist_keys (update n1 n2 substh) = oalist_keys (update n1 v vm1h)"
-    sorry
+  have One_one : "oalist_one_one (to_oalist (zip ns1t ns2t))"
+    using to_oalist_one_one[OF Dist1' Dist2'] Cons1.prems
+    by(auto)
 
-  have Conc3 : "oalist_one_one (update n1 n2 substh)"
-    sorry
+  have One_one_flip : "oalist_one_one (oalist_flip (to_oalist (zip ns1t ns2t)))"
+    using oalist_one_one_flip[OF One_one]
+    by auto
 
-  have Conc4 : "oalist_keys (oalist_flip (update n1 n2 substh)) = oalist_keys (update n2 v vm2h)"
-    sorry
-*)
+  have Len_tl : "length ns1t = length ns2t"
+    using Cons1.prems Cons2 by auto
+
+  have Notin2 : "ns2h \<notin> set ns2t"
+    using Cons1.prems Cons2
+    by(auto)
+
+  hence "ns2h \<notin> set (map snd (zip ns1t ns2t))"
+    using map_snd_zip[OF Len_tl]
+    by auto
+
+  hence "ns2h \<notin> snd ` set (zip ns1t ns2t)"
+    by auto
+ 
+  hence Notin2' : "ns2h \<notin> set (oalist_keys (oalist_flip (to_oalist (zip ns1t ns2t))))"
+    using oalist_keys_to_oalist_flip[OF Dist1' Dist2']
+    by(simp)
+
+  have Notin1 : "ns1h \<notin> set ns1t"
+    using Cons1.prems Cons2
+    by(auto)
+
+  hence "ns1h \<notin> set (map fst (zip ns1t ns2t))"
+    using map_fst_zip[OF Len_tl]
+    by auto
+
+  hence "ns1h \<notin> fst ` set (zip ns1t ns2t)"
+    by auto
+
+  hence Notin1' : "ns1h \<notin> set (oalist_keys (to_oalist (zip ns1t ns2t)))"
+    using oalist_keys_to_oalist[OF Dist1']
+    by(simp)
+
+  have Conc' : "oalist_flip (update ns1h ns2h (to_oalist (zip ns1t ns2t))) =
+    update ns2h ns1h (to_oalist (zip ns2t ns1t))"
+    using oalist_flip_update[OF One_one, OF Notin1' Notin2'] Cons1.prems Cons2 Tl(1)
+    by(auto)
 
   show ?case
-    using Cons1 Cons2 
-    apply(auto)
+    using Cons1.prems Cons2 Tl Conc'
+    by(auto)
+qed
+
+lemma strict_order_oalist_keys :
+  fixes l :: "('k :: linorder, 'v) oalist"
+  shows "strict_order (oalist_keys l)"
+  by(transfer; auto)
+
+lemma strict_order_unique_set :
+  assumes "strict_order l1"
+  assumes "strict_order l2"
+  assumes "set l1 = set l2"
+  shows "l1 = l2"
+  using assms
+proof(induction l1 arbitrary: l2)
+  case Nil
+  then show ?case
+    by(auto)
+next
+  case Cons1 : (Cons h1 t1)
+
+  obtain h2 t2 where Cons2 : "l2 = h2 # t2"
+    using Cons1
+    by(cases l2; auto)
+
+  have Ord_tl1 : "strict_order t1"
+    using strict_order_tl Cons1.prems
+    by auto
+
+  have Ord_tl2 : "strict_order t2"
+    using strict_order_tl Cons1.prems Cons2
+    by auto
+
+  have Dist1 : "distinct (h1 # t1)"
+    using strict_order_distinct[of "h1 # t1"] Cons1.prems
+    by auto
+
+  have Dist2 : "distinct (h2 # t2)"
+    using strict_order_distinct[of "h2 # t2"] Cons1.prems Cons2
+    by auto
+
+  show ?case
+  proof(cases "h1 = h2")
+    case True
+
+    have Set_eq_tl : "set t1 = set t2"
+      using Cons1.prems Cons2 True Dist1 Dist2
+      by(auto)
+
+    show ?thesis 
+      using Cons1.prems Cons2 True
+      using Cons1.IH[OF Ord_tl1 Ord_tl2 Set_eq_tl]
+      by(simp)
+  next
+    case Neq : False
+
+    have Sets_eq : "insert h1 (set t1) = insert h2 (set t2)"
+      using Cons1.prems Cons2
+      by(simp)
+
+    have H1_in2 : "h1 \<in> set t2"
+      using Sets_eq Neq Dist1
+      by(auto)
+
+    have H2_in1 : "h2 \<in> set t1"
+      using Sets_eq Neq Dist2
+      by(auto)
+
+    show ?thesis
+    proof(cases "h1 < h2")
+      case Lt : True
+
+      obtain ix where Ix : "t2 ! ix = h1" "ix < length t2"
+        using H1_in2
+        unfolding in_set_conv_nth
+        by auto
+
+      have Bad : "h2 < h1"
+        using strict_order_unfold[OF Cons1.prems(2), of "1 + ix" 0]
+          Ix Cons1.prems Cons2
+        by(auto)
+
+      then have False using Lt by auto
+
+      then show ?thesis by auto
+    next
+
+      case Gt' : False
+
+      have Gt : "h2 < h1"
+        using Neq Gt'
+        by auto
+
+      obtain ix where Ix : "t1 ! ix = h2" "ix < length t1"
+        using H2_in1
+        unfolding in_set_conv_nth
+        by auto
+
+      have Bad : "h1 < h2"
+        using strict_order_unfold[OF Cons1.prems(1), of "1 + ix" 0]
+          Ix Cons1.prems Cons2
+        by(auto)
+
+      then have False using Gt by auto
+
+      then show ?thesis by auto
+    qed
+  qed
 qed
 
 lemma alpha_equiv_varmap_extend :
@@ -1619,42 +2116,544 @@ next
     using Cons1.prems Cons2
     by auto
 
-(* need an alternate version of alpha_equiv_varmap_update
- * dealing with values not present? *)
+  have "\<exists>vmh'.
+     varmap_extend (Oalist.empty # vm1) ns1t = vmh' # vm1 \<and>
+     set (oalist_keys vmh') = set (oalist_keys (Oalist.empty :: (name, int) oalist)) \<union> set ns1t"
+    using varmap_extend_keys[of empty vm1 ns1t]
+    by auto
+
+  then obtain xh1 where Xh1 :
+    "(varmap_extend (Oalist.empty # vm1) ns1t) = xh1 # vm1"
+    "set (oalist_keys xh1) = set (oalist_keys (Oalist.empty :: (name, int) oalist)) \<union> set ns1t"
+    by auto
+
+  have "\<exists>vmh'.
+     varmap_extend (Oalist.empty # vm2) ns2t = vmh' # vm2 \<and>
+     set (oalist_keys vmh') = set (oalist_keys (Oalist.empty :: (name, int) oalist)) \<union> set ns2t"
+    using varmap_extend_keys[of empty vm2 ns2t]
+    by auto
+
+  then obtain xh2 where Xh2 :
+    "(varmap_extend (Oalist.empty # vm2) ns2t) = xh2 # vm2"
+    "set (oalist_keys xh2) = set (oalist_keys (Oalist.empty :: (name, int) oalist)) \<union> set ns2t"
+    by auto
+
+  have Vm_tl' :
+    "alpha_equiv_varmap (to_oalist (zip ns1t ns2t) # subst)
+     (xh1 # vm1)
+     (xh2 # vm2)"
+    using Vm_tl
+    unfolding Xh1(1) Xh2(1)
+    by auto
+
+  have Zip1 : "ns1t = map fst (zip ns1t ns2t)"
+    using map_fst_zip Cons1.prems Cons2
+    by(auto)
+
+  have Zip2 : "ns2t = map snd (zip ns1t ns2t)"
+    using map_fst_zip Cons1.prems Cons2
+    by(auto)
+
+  have One_one' : "oalist_one_one (to_oalist (zip ns1t ns2t))"
+    using to_oalist_one_one[of "(zip ns1t ns2t)"] Cons1.prems Cons2 Zip1 Zip2
+    by(auto)
+
+  have Keys1' : "set (oalist_keys (to_oalist (zip ns1t ns2t))) = set (map fst (zip ns1t ns2t))"
+    using oalist_keys_to_oalist[of "(zip ns1t ns2t)"] Zip1 Notin1
+    by(auto)
+
+  have Keys1x : "set (oalist_keys xh1) = set (map fst (zip ns1t ns2t))"
+    using Xh1 oalist_keys_empty Zip1
+    by(auto)
+
+  have Keys1x_eq_set : "set (oalist_keys (to_oalist (zip ns1t ns2t))) = set (oalist_keys xh1)"
+    using Keys1' Keys1x
+    by auto
+
+  have Keys1_eq : "(oalist_keys (to_oalist (zip ns1t ns2t))) = (oalist_keys xh1)"
+    using strict_order_unique_set[OF _ _ Keys1x_eq_set]
+    using strict_order_oalist_keys[of "(to_oalist (zip ns1t ns2t))"]
+    using strict_order_oalist_keys[of "xh1"]
+    by auto
+
+  have Keys2' : "set (oalist_keys (oalist_flip (to_oalist (zip ns1t ns2t)))) = (set (map snd (zip ns1t ns2t)))"
+    using oalist_keys_to_oalist_flip[of "(zip ns1t ns2t)"] Zip1 Zip2 Notin1 Notin2
+    by(auto)
+
+  have Keys2x : "set (oalist_keys xh2) = set (map snd (zip ns1t ns2t))"
+    using Xh2 oalist_keys_empty Zip2
+    by(auto)
+
+  have Keys2x_eq_set : "set (oalist_keys (oalist_flip (to_oalist (zip ns1t ns2t)))) = set (oalist_keys xh2)"
+    using Keys2' Keys2x
+    by auto
+
+  have Keys2_eq : "(oalist_keys (oalist_flip (to_oalist (zip ns1t ns2t)))) = (oalist_keys xh2)"
+    using strict_order_unique_set[OF _ _ Keys2x_eq_set]
+    using strict_order_oalist_keys[of "(oalist_flip (to_oalist (zip ns1t ns2t)))"]
+    using strict_order_oalist_keys[of "xh2"]
+    by auto
+
+  have Notin1' : "ns1h \<notin> set (oalist_keys xh1)"
+    using Xh1(2) Notin1 oalist_keys_empty
+    by(auto)
+
+  have Notin2' : "ns2h \<notin> set (oalist_keys xh2)"
+    using Xh2(2) Notin2 oalist_keys_empty
+    by(auto)
+
   show ?case using Vm_tl Cons1.prems Cons2 Vm_tl
     using varmap_extend_insert_swap[OF Notin1(1) Notin1(2)]
     using varmap_extend_insert_swap[OF Notin2(1) Notin2(2)]
-    apply(auto simp del: varmap_insert.simps)
-    sorry
+    using Xh1(1) Xh2(1)
+    using alpha_equiv_varmap_insert[OF Vm_tl' One_one' Keys1_eq Keys2_eq Notin1' Notin2', of 0]
+    by(auto simp del: varmap_insert.simps)
+qed
+
 (*
-(* need an assumption about one-one ness of ns1 and ns2? *)
-  show ?case
-  proof(cases "get (to_oalist (zip ns1t ns2t)) ns1h")
-    case None1 : None
+fix maps 1 and 2, assume they are alpha equiv
 
-    show ?thesis
-    proof(cases "get (oalist_flip (to_oalist (zip ns1t ns2t))) ns2h")
-      case None2 : None
-      then show ?thesis 
-        using Cons1.prems Cons2 None1
-        using alpha_equiv_varmap_update[OF _ Vm_tl, of ns1h ns2h]
-    apply(auto)
-        apply(auto)
-
-    next
-      case (Some a)
-      then show ?thesis sorry
-    qed
-      using None1 alpha_equiv_varmap_update[OF _ Vm_tl, of ns1h ns2h]
-      apply(auto)
-
-
-  show ?case using alpha_equiv_varmap_update[OF _ Vm_tl, of ns1h ns2h]
-    apply(auto)
-
-  then show ?case 
-    apply(auto)
+                have Vm_eq_pre_call : "alpha_equiv_varmap [to_oalist (zip (f1_args @ f1_rets) (f2_args @ f2_rets))] (varmap_inserts (varmap_extend [Oalist.empty] f1_rets) (zip f1_args res2))
+                  (varmap_inserts (varmap_extend [Oalist.empty] f2_rets) (zip f2_args res2))"
 *)
+
+lemma alpha_equiv_varmap_inserts :
+  assumes "alpha_equiv_varmap subst vm1 vm2"
+  assumes "length ns1 = length ns2"
+  assumes "distinct ns1"
+  assumes "distinct ns2"
+  shows "alpha_equiv_varmap (to_oalist (zip ns1 ns2) # subst)
+           (varmap_inserts (Oalist.empty # vm1) ns1)
+           (varmap_extend (Oalist.empty # vm2) ns2)"
+  using assms
+proof(induction ns1 arbitrary: subst vm1 vm2 ns2)
+  case Nil
+
+  have Keys : "oalist_keys Oalist.empty = oalist_keys Oalist.empty"
+    by(transfer; auto)
+
+  have One_one : "oalist_one_one Oalist.empty"
+    by(transfer; auto)
+
+  have Keys_flip : "oalist_keys (oalist_flip Oalist.empty) = oalist_keys Oalist.empty"
+    by(transfer; auto)
+
+  show ?case using Nil
+    using alpha_equiv_varmap'_empty Keys One_one Keys_flip
+    by(auto)
+next
+  case Cons1 : (Cons ns1h ns1t)
+
+  then obtain ns2h ns2t where Cons2 : "ns2 = ns2h # ns2t"
+    by(cases ns2; auto)
+
+  have Vm_tl : "alpha_equiv_varmap (to_oalist (zip ns1t ns2t) # subst) (varmap_extend (Oalist.empty # vm1) ns1t) (varmap_extend (Oalist.empty # vm2) ns2t)"
+    using Cons1.prems Cons2 Cons1.IH[OF Cons1.prems(1), of ns2t]
+    by(auto)
+
+  have Notin1 : "ns1h \<notin> set ns1t" "distinct ns1t"
+    using Cons1.prems
+    by auto
+
+  have Notin2 : "ns2h \<notin> set ns2t" "distinct ns2t"
+    using Cons1.prems Cons2
+    by auto
+
+  have "\<exists>vmh'.
+     varmap_extend (Oalist.empty # vm1) ns1t = vmh' # vm1 \<and>
+     set (oalist_keys vmh') = set (oalist_keys (Oalist.empty :: (name, int) oalist)) \<union> set ns1t"
+    using varmap_extend_keys[of empty vm1 ns1t]
+    by auto
+
+  then obtain xh1 where Xh1 :
+    "(varmap_extend (Oalist.empty # vm1) ns1t) = xh1 # vm1"
+    "set (oalist_keys xh1) = set (oalist_keys (Oalist.empty :: (name, int) oalist)) \<union> set ns1t"
+    by auto
+
+  have "\<exists>vmh'.
+     varmap_extend (Oalist.empty # vm2) ns2t = vmh' # vm2 \<and>
+     set (oalist_keys vmh') = set (oalist_keys (Oalist.empty :: (name, int) oalist)) \<union> set ns2t"
+    using varmap_extend_keys[of empty vm2 ns2t]
+    by auto
+
+  then obtain xh2 where Xh2 :
+    "(varmap_extend (Oalist.empty # vm2) ns2t) = xh2 # vm2"
+    "set (oalist_keys xh2) = set (oalist_keys (Oalist.empty :: (name, int) oalist)) \<union> set ns2t"
+    by auto
+
+  have Vm_tl' :
+    "alpha_equiv_varmap (to_oalist (zip ns1t ns2t) # subst)
+     (xh1 # vm1)
+     (xh2 # vm2)"
+    using Vm_tl
+    unfolding Xh1(1) Xh2(1)
+    by auto
+
+  have Zip1 : "ns1t = map fst (zip ns1t ns2t)"
+    using map_fst_zip Cons1.prems Cons2
+    by(auto)
+
+  have Zip2 : "ns2t = map snd (zip ns1t ns2t)"
+    using map_fst_zip Cons1.prems Cons2
+    by(auto)
+
+  have One_one' : "oalist_one_one (to_oalist (zip ns1t ns2t))"
+    using to_oalist_one_one[of "(zip ns1t ns2t)"] Cons1.prems Cons2 Zip1 Zip2
+    by(auto)
+
+  have Keys1' : "set (oalist_keys (to_oalist (zip ns1t ns2t))) = set (map fst (zip ns1t ns2t))"
+    using oalist_keys_to_oalist[of "(zip ns1t ns2t)"] Zip1 Notin1
+    by(auto)
+
+  have Keys1x : "set (oalist_keys xh1) = set (map fst (zip ns1t ns2t))"
+    using Xh1 oalist_keys_empty Zip1
+    by(auto)
+
+  have Keys1x_eq_set : "set (oalist_keys (to_oalist (zip ns1t ns2t))) = set (oalist_keys xh1)"
+    using Keys1' Keys1x
+    by auto
+
+  have Keys1_eq : "(oalist_keys (to_oalist (zip ns1t ns2t))) = (oalist_keys xh1)"
+    using strict_order_unique_set[OF _ _ Keys1x_eq_set]
+    using strict_order_oalist_keys[of "(to_oalist (zip ns1t ns2t))"]
+    using strict_order_oalist_keys[of "xh1"]
+    by auto
+
+  have Keys2' : "set (oalist_keys (oalist_flip (to_oalist (zip ns1t ns2t)))) = (set (map snd (zip ns1t ns2t)))"
+    using oalist_keys_to_oalist_flip[of "(zip ns1t ns2t)"] Zip1 Zip2 Notin1 Notin2
+    by(auto)
+
+  have Keys2x : "set (oalist_keys xh2) = set (map snd (zip ns1t ns2t))"
+    using Xh2 oalist_keys_empty Zip2
+    by(auto)
+
+  have Keys2x_eq_set : "set (oalist_keys (oalist_flip (to_oalist (zip ns1t ns2t)))) = set (oalist_keys xh2)"
+    using Keys2' Keys2x
+    by auto
+
+  have Keys2_eq : "(oalist_keys (oalist_flip (to_oalist (zip ns1t ns2t)))) = (oalist_keys xh2)"
+    using strict_order_unique_set[OF _ _ Keys2x_eq_set]
+    using strict_order_oalist_keys[of "(oalist_flip (to_oalist (zip ns1t ns2t)))"]
+    using strict_order_oalist_keys[of "xh2"]
+    by auto
+
+  have Notin1' : "ns1h \<notin> set (oalist_keys xh1)"
+    using Xh1(2) Notin1 oalist_keys_empty
+    by(auto)
+
+  have Notin2' : "ns2h \<notin> set (oalist_keys xh2)"
+    using Xh2(2) Notin2 oalist_keys_empty
+    by(auto)
+
+  show ?case using Vm_tl Cons1.prems Cons2 Vm_tl
+    using varmap_extend_insert_swap[OF Notin1(1) Notin1(2)]
+    using varmap_extend_insert_swap[OF Notin2(1) Notin2(2)]
+    using Xh1(1) Xh2(1)
+    using alpha_equiv_varmap_insert[OF Vm_tl' One_one' Keys1_eq Keys2_eq Notin1' Notin2', of 0]
+    by(auto simp del: varmap_insert.simps)
+qed
+
+lemma alpha_equiv_varmap_pop :
+  assumes H: "alpha_equiv_varmap (substh # subst) vm1 vm2"
+  shows "alpha_equiv_varmap subst (varmap_pop vm1) (varmap_pop vm2)"
+proof-
+  obtain vm1h vm1t where Vm1 : "vm1 = vm1h # vm1t"
+    using H
+    by(cases vm1; auto)
+
+  obtain vm2h vm2t where Vm2 : "vm2 = vm2h # vm2t"
+    using H
+    by(cases vm2; auto)
+
+  show "alpha_equiv_varmap subst (varmap_pop vm1)
+     (varmap_pop vm2)"
+    using Vm1 Vm2 H
+    by(auto)
+qed
+
+lemma alpha_equiv_fctx'_name :
+  assumes "alpha_equiv_fctx' ns ns_full ctx1 ctx2"
+  assumes "(f1, f2) \<in> set ns"
+
+  shows "(case get ctx1 f1 of
+    None \<Rightarrow> False
+    | Some fh1 \<Rightarrow>
+    (case get ctx2 f2 of
+     None \<Rightarrow> False
+     | Some fh2 \<Rightarrow>
+      (case (fh1, fh2) of
+        (Inl (Decl args1 rets1 body1), Inl (Decl args2 rets2 body2)) \<Rightarrow>
+          (length args1 = length args2 \<and>
+           length rets1 = length rets2 \<and>
+           distinct (args1 @ rets1) \<and>
+           distinct (args2 @ rets2) \<and>
+           alpha_equiv_stmt ns_full [to_oalist (zip (args1 @ rets1) (args2 @ rets2))] ctx1 ctx2 body1 body2)
+        | (Inr bh1, Inr bh2) \<Rightarrow>
+          \<comment> \<open>(bh1 = bh2)\<close> True
+        | (_, _) \<Rightarrow> False)))"
+  using assms
+proof(induction ns arbitrary: ns_full ctx1 ctx2 f1 f2)
+  case Nil
+  then show ?case by(auto)
+next
+  case (Cons nsh nst)
+
+  obtain nsh1 nsh2 where Nsh :
+    "nsh = (nsh1, nsh2)"
+    by(cases nsh; auto)
+
+  obtain fh1 where Fh1 : "get ctx1 nsh1 = Some fh1"
+    using Cons Nsh
+    by(cases "get ctx1 nsh1"; auto)
+
+  obtain fh2 where Fh2 : "get ctx2 nsh2 = Some fh2"
+    using Cons Nsh Fh1
+    by(cases "get ctx2 nsh2"; auto)
+
+  show ?case
+  proof(cases fh1)
+    case Inl1 : (Inl fh1d)
+
+    obtain args1 rets1 body1 where
+      Decl1 : "fh1d = Decl args1 rets1 body1"
+      by(cases fh1d; auto)
+
+    obtain fh2d where Inl2 : "fh2 = Inl fh2d"
+      using Cons Nsh Fh1 Fh2 Inl1 Decl1
+      by(cases fh2; auto)
+
+    obtain args2 rets2 body2 where
+      Decl2: "fh2d = Decl args2 rets2 body2"
+      by(cases fh2d; auto)
+
+
+    show ?thesis 
+      using Cons Nsh Fh1 Fh2 Inl1 Decl1 Inl2 Decl2
+      by(auto)
+  next
+    case Inr1 : (Inr err1)
+    then show ?thesis 
+      using Cons Nsh Fh1 Fh2
+      by(cases fh2; auto)
+  qed
+qed
+
+
+lemma oacons_impl_of : 
+  fixes l :: "('k :: linorder, 'v) oalist"
+  assumes "oacons hk hv t = Some l"
+  shows "impl_of l = (hk, hv) # (impl_of t)"
+  using assms
+proof(transfer)
+  fix t :: "('k * 'v) list"
+  fix hk hv l
+  show "strict_order (map fst t) \<Longrightarrow>
+       strict_order (map fst l) \<Longrightarrow>
+       oacons' hk hv t = Some l \<Longrightarrow>
+       l = (hk, hv) # t"
+    by(cases t; auto split: if_splits)
+qed
+
+lemma oacons_update :
+  fixes l :: "('k :: linorder, 'v) oalist"
+  assumes "oacons hk hv t = Some l"
+  shows "update hk hv t = l"
+  using assms
+proof(transfer)
+  fix hk hv
+  fix t l :: "('k * 'v) list"
+
+  assume Ord1 : "strict_order (map fst t)"
+  assume Ord2 : "strict_order (map fst l)"
+  assume Oacons : "oacons' hk hv t = Some l"
+  show "str_ord_update hk hv t = l"
+  proof(cases t)
+    case Nil
+    then show ?thesis 
+      using Oacons
+      by auto
+  next
+    case (Cons lh' lt)
+
+    obtain lh'k lh'v where Lh' :
+      "lh' = (lh'k, lh'v)"
+      by(cases lh'; auto)
+
+    show ?thesis using Cons Oacons Lh'
+      by(auto)
+  qed
+qed
+
+lemma to_oalist_impl_of : 
+  fixes l :: "('k :: linorder, 'v) oalist"
+  assumes "l' = impl_of l"
+  shows "to_oalist l' = l"
+  using assms
+proof(induction l' arbitrary: l)
+  case Nil
+  then show ?case 
+    by(clarsimp;transfer; auto)
+next
+  case (Cons l'h l't)
+
+  obtain l'hk l'hv where L'h :
+    "l'h = (l'hk, l'hv)"
+    by(cases l'h; auto)
+
+  consider (1) "l = empty"
+    | (2) lhk lhv lt where
+      "oacons lhk lhv lt = Some l"
+    using oalist_cases[of l]
+    by auto
+  then show ?case
+  proof cases
+    case 1
+
+    have "l'h # l't = impl_of Oalist.empty"
+      using Cons 1 by auto
+
+    then have False
+      by (transfer; auto)
+
+    then show ?thesis by auto
+  next
+    case 2
+
+    have Eqs :
+      "l'hk = lhk" "l'hv = lhv" "l't = impl_of lt"
+      using oacons_impl_of[OF 2] Cons.prems L'h
+      by(auto)
+
+    have L_unfold : "(lhk, lhv) # impl_of lt = impl_of l"
+      using Cons.prems L'h Cons.IH[OF Eqs(3)] Eqs
+      by(auto)
+
+    have Conc' : "update lhk lhv lt = l"
+      using oacons_update[OF 2]
+      by auto
+
+    show ?thesis using Cons.prems L'h Cons.IH[OF Eqs(3)]
+        sym[OF L_unfold] Conc'
+      by(auto)
+  qed
+qed
+
+
+lemma alpha_equiv_fctx_name :
+  assumes Hfctx : "alpha_equiv_fctx (impl_of fsubst) ctx1 ctx2"
+  assumes Hname' : "alpha_equiv_name' fsubst f1 f2"
+
+  shows "(case get ctx1 f1 of
+    None \<Rightarrow> False
+    | Some fh1 \<Rightarrow>
+    (case get ctx2 f2 of
+     None \<Rightarrow> False
+     | Some fh2 \<Rightarrow>
+      (case (fh1, fh2) of
+        (Inl (Decl args1 rets1 body1), Inl (Decl args2 rets2 body2)) \<Rightarrow>
+          (length args1 = length args2 \<and>
+           length rets1 = length rets2 \<and>
+           distinct (args1 @ rets1) \<and>
+           distinct (args2 @ rets2) \<and>
+           alpha_equiv_stmt (to_oalist (impl_of fsubst)) [to_oalist (zip (args1 @ rets1) (args2 @ rets2))] ctx1 ctx2 body1 body2)
+        | (Inr bh1, Inr bh2) \<Rightarrow>
+          \<comment> \<open>(bh1 = bh2)\<close> True
+        | (_, _) \<Rightarrow> False)))"
+  using assms
+proof-
+
+  have Fctx' : " alpha_equiv_fctx' (impl_of fsubst) (to_oalist (impl_of fsubst)) ctx1 ctx2"
+    using Hfctx
+    by(auto simp add: alpha_equiv_fctx_def)
+
+  hence Fctx'' : "alpha_equiv_fctx' (impl_of fsubst) fsubst ctx1 ctx2"
+    using to_oalist_impl_of[of "impl_of fsubst" fsubst]
+    by(auto simp add: alpha_equiv_fctx_def)
+
+  have Get : "get fsubst f1 = Some f2"
+    using Hname'
+    by(auto simp add: alpha_equiv_name'_def split: option.splits)
+
+  then have In : "(f1, f2) \<in> set (impl_of fsubst)"
+  proof(transfer)
+    fix fsubst :: "(name* name) list"
+    fix f1 f2
+    assume Mapof : "map_of fsubst f1 = Some f2" 
+    show "(f1, f2) \<in> set fsubst"
+      using map_of_SomeD[OF Mapof]
+      by auto
+  qed
+
+  show ?thesis
+    using Hfctx Hname'
+      alpha_equiv_fctx'_name[OF Fctx' In]
+    by(auto)
+qed
+
+lemma varmap_gets_length : 
+  assumes "varmap_gets vm ns = Some vals"
+  shows "length ns = length vals"
+  using assms
+proof(induction ns arbitrary: vm vals)
+  case Nil
+  then show ?case by auto
+next
+  case Cons1 : (Cons nsh nst)
+
+  obtain vmh vmt where Cons2 : "vm = vmh # vmt"
+    using Cons1
+    by(cases vm; auto)
+
+  show ?case
+  proof(cases "get vmh nsh")
+    case None
+
+    obtain vh where Vh : "varmap_get vmt nsh = Some vh"
+      using Cons1 Cons2 None
+      by(cases "varmap_get vmt nsh"; auto)
+
+    obtain vt where Vt : "varmap_gets (vmh # vmt) nst = Some vt"
+      using Cons1 Cons2 None Vh
+      by(cases "varmap_gets (vmh # vmt) nst"; auto)
+
+    then show ?thesis using Cons1 Cons2 None Vh Vt
+      by(auto)
+  next
+    case (Some vh)
+
+    obtain vt where Vt : "varmap_gets (vmh # vmt) nst = Some vt"
+      using Cons1 Cons2 Some
+      by(cases "varmap_gets (vmh # vmt) nst"; auto)
+
+    show ?thesis using Cons1 Cons2 Some Vt
+      by(auto)
+  qed
+qed
+
+lemma alpha_equiv_varmap_gets_names :
+  assumes "alpha_equiv_varmap subst vm1 vm2"
+  assumes "list_all2 (alpha_equiv_name subst) vs1 vs2"
+  shows "varmap_gets vm1 vs1 = varmap_gets vm2 vs2"
+  using assms
+proof(induction vs1 arbitrary: subst vm1 vm2 vs2)
+  case Nil
+  then show ?case
+    by auto
+next
+  case Cons1 : (Cons v1h v1t)
+
+  obtain v2h v2t where Cons2 : "vs2 = v2h # v2t"
+    using Cons1.prems
+    by(cases vs2; auto)
+
+  have Eqv_h : "alpha_equiv_name subst v1h v2h"
+    using Cons1.prems Cons2
+    by auto
+
+  show ?case using Cons1.prems Cons2
+      alpha_equiv_varmap_name[OF Cons1.prems(1) Eqv_h]
+      Cons1.IH[OF Cons1.prems(1), of v2t]
+    by(auto split: option.splits)
 qed
 
 lemma alpha_equiv_eval_correct:
@@ -1829,10 +2828,13 @@ next
             "res2_p = (res2_vm, res2_g)"
             by(cases res2_p; auto)
 
+          have Vmeq_result : "alpha_equiv_varmap (to_oalist (zip ns1 ns2) # subst) res1_vm res2_vm"
+            using SB1 SB2 Hvm IH3[OF Vm_extend Hfctx Bodies, of g] Some1 Ok1 Res1 Some2 Ok2 Res2
+            by(auto)
+
           have Pop : "alpha_equiv_varmap subst (varmap_pop res1_vm) (varmap_pop res2_vm)"
-            using SB1 SB2 Heqv Some1 Some2 Ok1 Ok2 Res1 Res2 Hvm
-            apply(auto)
-            sorry (* lemma *)
+            using alpha_equiv_varmap_pop[OF Vmeq_result]
+            by(auto)
 
           show ?thesis 
             using SB1 SB2 Heqv Some1 Some2 Ok1 Res1 Ok2 Res2 IH3[OF Vm_extend Hfctx Bodies, of g]
@@ -2164,11 +3166,11 @@ next
           using EPrim1 EPrim2 Heqv Some1 Args
           by(cases "eval_expr1s vm2 args2"; auto)
 
-
         show ?thesis 
           sorry
       qed
     next
+
       case EFun1 : (EFun f1 args1)
       obtain f2 args2 where EFun2 : "expr2 = EFun f2 args2"
         using EFun1 Heqv
@@ -2177,6 +3179,10 @@ next
       have Args : "eval_expr1s vm1 args1 = eval_expr1s vm2 args2"
         using EFun1 EFun2 Heqv alpha_equiv_eval_expr1s_correct[OF Hvm, of args1 args2]
         by auto
+
+      have Fname : "alpha_equiv_name' fsubst f1 f2"
+        using EFun1 EFun2 Args Heqv
+        by(auto)
 
       show ?thesis 
       proof(cases "eval_expr1s vm1 args1")
@@ -2192,13 +3198,329 @@ next
           using EFun1 EFun2 Heqv Some1 Args
           by(cases "eval_expr1s vm2 args2"; auto)
 
-
         show ?thesis 
-          using EFun1 EFun2 Args Some1 Some2 Heqv
-          apply(auto)
-          sorry
-      qed
+        proof(cases "get ctx1 f1")
+          case None_get_ctx1 : None
 
+
+          show ?thesis
+          proof(cases "get ctx2 f2")
+            case None_get_ctx2 : None
+            show ?thesis
+              using EFun1 EFun2 Args Some1 Some2 Heqv None_get_ctx1 None_get_ctx2
+              by auto
+          next
+            case Some_get_ctx2 : (Some fres2)
+            then show ?thesis 
+              using EFun1 EFun2 Args Some1 Some2 Heqv Hfctx None_get_ctx1 Some_get_ctx2
+              using alpha_equiv_fctx_name[OF Hfctx Fname]
+              by(auto)
+          qed
+        next
+          case Some_get_ctx1 : (Some fres1)
+
+          show ?thesis
+          proof(cases "get ctx2 f2")
+            case None_get_ctx2 : None
+            show ?thesis
+              using EFun1 EFun2 Args Some1 Some2 Heqv Some_get_ctx1 None_get_ctx2
+              using alpha_equiv_fctx_name[OF Hfctx Fname]
+              by(auto)
+          next
+            case Some_get_ctx2 : (Some fres2)
+
+            show ?thesis
+            proof(cases fres1)
+              case Inl1 : (Inl decl1)
+
+              obtain f1_args f1_rets f1_body where
+                Decl1 : "decl1 = Decl f1_args f1_rets f1_body"
+                by(cases decl1; auto)
+
+              show ?thesis
+              proof(cases fres2)
+                case Inl2 : (Inl decl2)
+
+                obtain f2_args f2_rets f2_body where
+                  Decl2 : "decl2 = Decl f2_args f2_rets f2_body"
+                  by(cases decl2; auto)
+
+                have Args_len_eq : "length f1_args = length f2_args"
+                  using alpha_equiv_fctx_name[OF Hfctx Fname]
+                    EFun1 EFun2 Args Some1 Some2 Heqv Some_get_ctx1 Some_get_ctx2 Inl1 Decl1 Inl2 Decl2
+                  by(auto)
+
+                have Rets_len_eq : "length f1_rets = length f2_rets"
+                  using alpha_equiv_fctx_name[OF Hfctx Fname]
+                    EFun1 EFun2 Args Some1 Some2 Heqv Some_get_ctx1 Some_get_ctx2 Inl1 Decl1 Inl2 Decl2
+                  by(auto)
+
+                have Args_rets_dist1 :
+                  "distinct (f1_args @ f1_rets)"
+                  using alpha_equiv_fctx_name[OF Hfctx Fname]
+                    EFun1 EFun2 Args Some1 Some2 Heqv Some_get_ctx1 Some_get_ctx2 Inl1 Decl1 Inl2 Decl2
+                  by(auto)
+
+                have Args_rets_dist2 :
+                  "distinct (f2_args @ f2_rets)"
+                  using alpha_equiv_fctx_name[OF Hfctx Fname]
+                    EFun1 EFun2 Args Some1 Some2 Heqv Some_get_ctx1 Some_get_ctx2 Inl1 Decl1 Inl2 Decl2
+                  by(auto)
+
+                have Vm_eq_pre_call : "alpha_equiv_varmap [to_oalist (zip (f1_args @ f1_rets) (f2_args @ f2_rets))] (varmap_inserts (varmap_extend [Oalist.empty] f1_rets) (zip f1_args res2))
+                  (varmap_inserts (varmap_extend [Oalist.empty] f2_rets) (zip f2_args res2))"
+                  apply(simp)
+                  (* alpha_equiv_varmap_updates, applied to a varmap with only args and rets *)
+                  sorry
+
+                have Bodies : "alpha_equiv_stmt (to_oalist (impl_of fsubst)) [to_oalist (zip (f1_args @ f1_rets) (f2_args @ f2_rets))] ctx1 ctx2 f1_body f2_body"
+                  using alpha_equiv_fctx_name[OF Hfctx Fname] Some_get_ctx1 Some_get_ctx2 Inl1 Inl2 Decl1 Decl2
+                  by(auto)
+
+                hence Bodies' : "alpha_equiv_stmt fsubst [to_oalist (zip (f1_args @ f1_rets) (f2_args @ f2_rets))] ctx1 ctx2 f1_body f2_body"
+                  using to_oalist_impl_of[of "impl_of fsubst" fsubst]
+                  by(auto)
+
+                have Body_results :
+                  "alpha_equiv_results [to_oalist (zip (f1_args @ f1_rets) (f2_args @ f2_rets))]
+                    (eval_statement n' ctx1 f1_body (varmap_inserts (varmap_extend [Oalist.empty] f1_rets) (zip f1_args res2)) g)
+                    (eval_statement n' ctx2 f2_body (varmap_inserts (varmap_extend [Oalist.empty] f2_rets) (zip f2_args res2)) g)"
+                  using IH1[OF Vm_eq_pre_call Hfctx Bodies']
+                  by auto
+
+                show ?thesis
+                proof(cases "eval_statement n' ctx1 f1_body (varmap_inserts (varmap_extend [Oalist.empty] f1_rets) (zip f1_args res2)) g")
+                  case None_eval_body1 : None
+
+                  show ?thesis
+                  proof(cases "(eval_statement n' ctx2 f2_body (varmap_inserts (varmap_extend [Oalist.empty] f2_rets) (zip f2_args res2)) g)")
+                    case None_eval_body2 : None
+                    then show ?thesis 
+                      using EFun1 EFun2 Args Some1 Some2 Heqv Some_get_ctx1 Some_get_ctx2 Inl1 Decl1 Inl2 Decl2 None_eval_body1 Args_len_eq
+                      by(auto)
+                  next
+                    case Some_eval_body2 : (Some bres2)
+                    then show ?thesis 
+                      using EFun1 EFun2 Args Some1 Some2 Heqv Some_get_ctx1 Some_get_ctx2 Inl1 Decl1 Inl2 Decl2 None_eval_body1 Args_len_eq
+                      using Body_results
+                      by(auto)
+                  qed
+                next
+                  case Some_eval_body1 : (Some bres1)
+
+                  show ?thesis
+                  proof(cases bres1)
+                    case Ok_eval_body1 : (Ok bres1')
+
+                    obtain vmfinal1 gfinal1 where Bres1' : "bres1' = (vmfinal1, gfinal1)"
+                      by(cases bres1'; auto)
+
+                    show ?thesis
+                    proof(cases "(eval_statement n' ctx2 f2_body (varmap_inserts (varmap_extend [Oalist.empty] f2_rets) (zip f2_args res2)) g)")
+                      case None_eval_body2 : None
+                      then show ?thesis
+                        using EFun1 EFun2 Args Some1 Some2 Heqv Some_get_ctx1 Some_get_ctx2 Inl1 Decl1 Inl2 Decl2 Some_eval_body1 Args_len_eq
+                        using Body_results
+                        by(auto)
+                    next
+                      case Some_eval_body2 : (Some bres2)
+    
+                      show ?thesis
+                      proof(cases bres2)
+                        case Ok_eval_body2 : (Ok bres2')
+    
+                        obtain vmfinal2 gfinal2 where Bres2' : "bres2' = (vmfinal2, gfinal2)"
+                          by(cases bres2'; auto)
+
+                        have Vm_eq_post_call : 
+                          "alpha_equiv_varmap [to_oalist (zip f1_args f2_args @ zip f1_rets f2_rets)] vmfinal1
+                               vmfinal2"
+                          using EFun1 EFun2 Args Some1 Some2 Heqv Some_get_ctx1 Some_get_ctx2 Inl1 Decl1 Inl2 Decl2 Some_eval_body1 Ok_eval_body1 Bres1' Some_eval_body2  Ok_eval_body2 Bres2'
+                          using Body_results Args_len_eq
+                          by(auto)
+
+                        have Rets_names : "list_all2 (alpha_equiv_name [to_oalist (zip (f1_args @ f1_rets) (f2_args @ f2_rets))]) f1_rets f2_rets"
+                        proof(rule list_all2_all_nthI)
+                          show "length f1_rets = length f2_rets"
+                            using Rets_len_eq
+                            by auto
+                        next
+                          fix n
+                          assume N : "n < length f1_rets"
+
+                          have Dist1 : "distinct (map fst (zip f1_args f2_args @ zip f1_rets f2_rets))"
+                            using EFun1 EFun2 Args Some1 Some2 Heqv Some_get_ctx1 Some_get_ctx2 Inl1 Decl1 Inl2 Decl2 Some_eval_body1 Ok_eval_body1 Bres1' Some_eval_body2  Ok_eval_body2 Bres2'
+                            using alpha_equiv_fctx_name[OF Hfctx Fname]
+                            by(auto)
+
+                          have Dist2 : "distinct (map fst (zip f2_args f1_args @ zip f2_rets f1_rets))"
+                            using EFun1 EFun2 Args Some1 Some2 Heqv Some_get_ctx1 Some_get_ctx2 Inl1 Decl1 Inl2 Decl2 Some_eval_body1 Ok_eval_body1 Bres1' Some_eval_body2  Ok_eval_body2 Bres2'
+                            using alpha_equiv_fctx_name[OF Hfctx Fname]
+                            by(auto)
+
+                          have Get1 : "get (to_oalist (zip f1_args f2_args @ zip f1_rets f2_rets)) (f1_rets ! n) = map_of (zip f1_args f2_args @ zip f1_rets f2_rets) (f1_rets ! n)"
+                            using get_to_oalist[OF Dist1]
+                            by auto
+
+                          have Get1' : "map_of (zip f1_args f2_args @ zip f1_rets f2_rets) (f1_rets ! n) = Some (f2_rets ! n)"
+                            using Args_len_eq Rets_len_eq Dist1
+                            (* via sledgehammer *)
+                            by (auto; smt (z3) N dom_map_of_zip map_add_comm map_add_find_right map_of_zip_nth)
+
+                          have Flip : "(oalist_flip (to_oalist (zip f1_args f2_args @ zip f1_rets f2_rets))) =
+                            to_oalist (zip f2_args f1_args @ zip f2_rets f1_rets)"
+                            using to_oalist_flip_zip[OF Args_rets_dist1 Args_rets_dist2] Args_len_eq Rets_len_eq
+                            by(auto)
+
+                          have Get2 : "get (oalist_flip (to_oalist (zip f1_args f2_args @ zip f1_rets f2_rets))) (f2_rets ! n) = 
+                                       map_of (zip f2_args f1_args @ zip f2_rets f1_rets) (f2_rets ! n)"
+                            using Flip get_to_oalist[OF Dist2]
+                            by(auto)
+
+                          have Get2' : "map_of (zip f2_args f1_args @ zip f2_rets f1_rets) (f2_rets ! n) = Some (f1_rets ! n)"
+                            using Args_len_eq Rets_len_eq Dist2
+                            (* via sledgehammer *)
+                            by (auto; smt (z3) N dom_map_of_zip map_add_comm map_add_find_right map_of_zip_nth)
+
+                          show "alpha_equiv_name
+                            [to_oalist (zip (f1_args @ f1_rets) (f2_args @ f2_rets))]
+                            (f1_rets ! n) (f2_rets ! n)"
+                            using alpha_equiv_fctx_name[OF Hfctx Fname] Some_get_ctx1 Some_get_ctx2 Inl1 Inl2 Decl1 Decl2
+                            using Get1 Get1' Get2 Get2'
+                            by(auto)
+                        qed
+
+                        show ?thesis
+                        proof(cases "varmap_gets vmfinal1 f1_rets")
+                          case None_returns1 : None
+                          then show ?thesis 
+                            using EFun1 EFun2 Args Some1 Some2 Heqv Some_get_ctx1 Some_get_ctx2 Inl1 Decl1 Inl2 Decl2 Some_eval_body1 Ok_eval_body1 Bres1' Some_eval_body2  Ok_eval_body2 Bres2'
+                            using Body_results Args_len_eq
+                            using alpha_equiv_varmap_gets_names[OF Vm_eq_post_call, of f1_rets f2_rets ] Rets_names
+                            by(auto)
+
+                        next
+                          case Some_returns1 : (Some retvals1)
+                          show ?thesis
+                          proof(cases "varmap_gets vmfinal2 f2_rets")
+                            case None_returns2 : None
+
+                            then show ?thesis
+                              using EFun1 EFun2 Args Some1 Some2 Heqv Some_get_ctx1 Some_get_ctx2 Inl1 Decl1 Inl2 Decl2 Some_eval_body1 Ok_eval_body1 Bres1' Some_eval_body2  Ok_eval_body2 Bres2'
+                              using Body_results Args_len_eq
+                              using alpha_equiv_varmap_gets_names[OF Vm_eq_post_call, of f1_rets f2_rets ] Rets_names
+                              by(auto)
+
+                          next
+                            case Some_returns2 : (Some retvals2)
+
+                            have Fname : "alpha_equiv_name' fsubst f1 f2"
+                              using EFun1 EFun2 Args Some1 Some2 Heqv Some_get_ctx1 Some_get_ctx2 Inl1 Decl1 Inl2 Decl2
+                                Some_eval_body1 Ok_eval_body1 Bres1' Some_eval_body2 Ok_eval_body2 Bres2' Some_returns1 Some_returns2
+                              by(auto)
+
+                            have Rets_len_eq1 : "length retvals1 = length f1_rets"
+                              using EFun1 EFun2 Args Some1 Some2 Heqv Some_get_ctx1 Some_get_ctx2 Inl1 Decl1 Inl2 Decl2
+                              Some_eval_body1 Ok_eval_body1 Bres1' Some_eval_body2 Ok_eval_body2 Bres2' Some_returns1 Some_returns2
+                              using varmap_gets_length
+                              by(auto)
+
+                            have Rets_len_eq2 : "length retvals2 = length f2_rets"
+                              using EFun1 EFun2 Args Some1 Some2 Heqv Some_get_ctx1 Some_get_ctx2 Inl1 Decl1 Inl2 Decl2
+                              Some_eval_body1 Ok_eval_body1 Bres1' Some_eval_body2 Ok_eval_body2 Bres2' Some_returns1 Some_returns2
+                              using varmap_gets_length
+
+                              by(auto)
+
+                            have Retvals_eq : "retvals1 = retvals2"
+                              using EFun1 EFun2 Args Some1 Some2 Heqv Some_get_ctx1 Some_get_ctx2 Inl1 Decl1 Inl2 Decl2
+                                Some_eval_body1 Ok_eval_body1 Bres1' Some_eval_body2 Ok_eval_body2 Bres2' Some_returns1 Some_returns2
+                              using Body_results Args_len_eq
+                              using alpha_equiv_varmap_gets_names[OF Vm_eq_post_call , of f1_rets f2_rets] Rets_names
+                              by(auto)
+
+                            show ?thesis
+                              using EFun1 EFun2 Args Some1 Some2 Heqv Some_get_ctx1 Some_get_ctx2 Inl1 Decl1 Inl2 Decl2
+                                Some_eval_body1 Ok_eval_body1 Bres1' Some_eval_body2 Ok_eval_body2 Bres2' Some_returns1 Some_returns2
+                              using Body_results Args_len_eq Rets_len_eq1 Rets_len_eq2 Retvals_eq
+                              by(auto)
+                          qed
+                        qed
+                      next
+                        case Error_eval_body2 : (Error err2)
+
+                        then show ?thesis
+                          using EFun1 EFun2 Args Some1 Some2 Heqv Some_get_ctx1 Some_get_ctx2 Inl1 Decl1 Inl2 Decl2
+                            Some_eval_body1 Ok_eval_body1 Bres1' Some_eval_body2
+                          using Body_results
+                          by(auto)
+                      qed
+                    qed
+                  next
+                    case Error_eval_body1 : (Error err1)
+
+                    show ?thesis
+                    proof(cases "(eval_statement n' ctx2 f2_body (varmap_inserts (varmap_extend [Oalist.empty] f2_rets) (zip f2_args res2)) g)")
+                      case None_eval_body2 : None
+                      then show ?thesis
+                        using EFun1 EFun2 Args Some1 Some2 Heqv Some_get_ctx1 Some_get_ctx2 Inl1 Decl1 Inl2 Decl2 Some_eval_body1 Args_len_eq
+                        using Body_results
+                        by(auto)
+                    next
+                      case Some_eval_body2 : (Some bres2)
+    
+                      show ?thesis
+                      proof(cases bres2)
+                        case Ok_eval_body2 : (Ok bres2')
+    
+                        obtain vmfinal2 gfinal2 where Bres2' : "bres2' = (vmfinal2, gfinal2)"
+                          by(cases bres2'; auto)
+
+                        show ?thesis
+                          using EFun1 EFun2 Args Some1 Some2 Heqv Some_get_ctx1 Some_get_ctx2 Inl1 Decl1 Inl2 Decl2 Some_eval_body1 Args_len_eq
+                          using Error_eval_body1 Some_eval_body2 Ok_eval_body2
+                          using Body_results
+                          by(auto)
+                      next
+                        case Error_eval_body2 : (Error err2)
+
+                        show ?thesis
+                          using EFun1 EFun2 Args Some1 Some2 Heqv Some_get_ctx1 Some_get_ctx2 Inl1 Decl1 Inl2 Decl2 Some_eval_body1 Args_len_eq
+                          using Error_eval_body1 Some_eval_body2 Error_eval_body2
+                          using Body_results
+                          by(auto)
+                      qed
+                    qed
+                  qed
+                qed
+              next
+                case Inr2 : (Inr err2)
+
+                show ?thesis
+                  using alpha_equiv_fctx_name[OF Hfctx Fname]
+                  using EFun1 EFun2 Args Some1 Some2 Heqv Some_get_ctx1 Some_get_ctx2 Inl1 Decl1 Inr2
+                  by(auto)
+              qed
+            next
+              case Inr1 : (Inr err1)
+              show ?thesis
+              proof(cases fres2)
+                case Inl2 : (Inl decl2)
+                show ?thesis
+                  using alpha_equiv_fctx_name[OF Hfctx Fname]
+                  using EFun1 EFun2 Args Some1 Some2 Heqv Some_get_ctx1 Some_get_ctx2 Inr1 Inl2
+                  by(auto)
+              next
+                case Inr2 : (Inr err2)
+                show ?thesis
+                  using alpha_equiv_fctx_name[OF Hfctx Fname]
+                  using EFun1 EFun2 Args Some1 Some2 Heqv Some_get_ctx1 Some_get_ctx2 Inr1 Inr2
+                  by(auto)
+              qed
+            qed
+          qed
+        qed
+      qed
     qed
   qed
 
